src/temporal_logic/refinement/many_to_many.lean
@@ -15,126 +15,133 @@ namespace many_to_many
 section
 open fairness
 parameters {α : Type u} {β : Type u₀} {γ : Type u₁ }
-parameters {aevt : Type u₂} {cevt : Type u₃}
-parameters {p : pred' (γ×α)} {q : pred' (γ×β)}
-parameters (A : aevt → act (γ×α)) (C : cevt → act (γ×β))
-parameters {cs₀ fs₀ : aevt → pred' (γ×α)} {cs₁ fs₁ : cevt → pred' (γ×β)}
+parameters {m₀ : mch (γ×α)} {m₁ : mch (γ×β)}
+local notation `p` := m₀.init
+local notation `q` := m₁.init
+local notation `aevt` := m₀.evt
+local notation `cevt` := m₁.evt
+local notation `cs₀` := m₀.cs
+local notation `fs₀` := m₀.fs
+local notation `cs₁` := m₁.cs
+local notation `fs₁` := m₁.fs
+local notation `A` := m₀.A
+local notation `C` := m₁.A
+local notation `ae`  := m₀.event
+local notation `ce`  := m₁.event
+local notation `ce'` := m₁.event' (option aevt)
+-- local notation `Next₀` := m₀.effect
+-- local notation `Next₁` := m₁.effect
+
+
 parameters (J : pred' (γ×α×β))
-parameters (Jₐ : pred' (γ×α))
-parameter ref : aevt → cevt → Prop
-parameter wit : Π a, subtype (ref a) → cpred
+parameter ref : option aevt → option cevt → Prop
+parameter wit : Π a : aevt, subtype (λ c : cevt, ref a c) → cpred
 
 open prod
 
 def C' (e : cevt) : act (cevt×γ×β) :=
 λ ⟨sch,s⟩ ⟨_,s'⟩, sch = e ∧ C e s s'
 
-abbreviation ae (i : aevt) : event (γ×α) := ⟨cs₀ i,fs₀ i,A i⟩
-abbreviation ce (i : cevt) : event (γ×β) := ⟨cs₁ i,fs₁ i,C i⟩
 
-abbreviation ae' (i : aevt) : event (γ×α×aevt) :=
-{ p := cs₀ i!⟨prod.map_right fst⟩
-, q := fs₀ i!⟨prod.map_right fst⟩
-, A := λ s s', s.2.2 = i ∧ (A i on prod.map_right fst) s s' }
-abbreviation ce' (i : cevt) (j : aevt) : event (γ×β×cevt×aevt) :=
-{ p := cs₁ i!⟨prod.map_right fst⟩
-, q := fs₁ i!⟨prod.map_right fst⟩
-, A := λ ⟨o,v,ce,_⟩ ⟨o',v',_,ae'⟩, ae' = j ∧ ce = i ∧ C i (o,v) (o',v') }
+-- #check (_ × _) × _
+-- abbreviation ae' (i : aevt) : event (γ×α×aevt) :=
+-- { p := cs₀ i!⟨prod.map_right fst⟩
+-- , q := fs₀ i!⟨prod.map_right fst⟩
+-- , A := λ s s', s.2.2 = i ∧ (A i on prod.map_right fst) s s' }
+-- abbreviation ce' (i : cevt) (j : aevt) : event (γ×β×(cevt×aevt)) :=
+-- { p := cs₁ i!⟨prod.map_right fst⟩
+-- , q := fs₁ i!⟨prod.map_right fst⟩
+-- , A := λ ⟨o,v,ce,_⟩ ⟨o',v',_,ae'⟩, ae' = j ∧ ce = i ∧ C i (o,v) (o',v') }
 
 section specs
 
-parameters p q cs₀ fs₀ cs₁ fs₁
+-- parameters p q cs₀ fs₀ cs₁ fs₁
 
-def SPEC₀.saf' (v : tvar α) (o : tvar γ) (sch : tvar aevt) : cpred :=
-p ! ⦃ o,v ⦄ ⋀
-◻(∃∃ i, ⊙sch ≃ ↑i ⋀ ⟦ o,v | A i ⟧)
+def SPEC₀.saf' (v : tvar α) (o : tvar γ) (sch : tvar (option aevt)) : cpred :=
+m₀.spec_saf_sch ⦃o,v⦄ (⊙sch)
 
 def SPEC₀ (v : tvar α) (o : tvar γ) : cpred :=
-spec p cs₀ fs₀ A ⦃o,v⦄
+m₀.spec ⦃ o,v ⦄
 
 def SPEC₁ (v : tvar β) (o : tvar γ) : cpred :=
-spec q cs₁ fs₁ C ⦃o,v⦄
+m₁.spec ⦃ o,v ⦄
 
-def SPEC₂ (v : tvar β) (o : tvar γ) (s : tvar cevt) : cpred :=
-spec_sch q cs₁ fs₁ C ⦃o,v⦄ s
+def SPEC₂ (v : tvar β) (o : tvar γ) (s : tvar (option cevt)) : cpred :=
+m₁.spec_sch ⦃o,v⦄ s
 
 end specs
 
-parameters [inh_α : inhabited α]
-           [inh_cevt : inhabited cevt]
+parameters [inh_cevt : inhabited cevt]
            [inh_aevt : inhabited aevt]
 
-parameter Hc2a : ∀ ce : cevt, ∃ ae : aevt, ref ae ce
+-- parameter Hc2a : ∀ ce : cevt, ∃ ae : aevt, ref ae ce
 
-parameter init_Jₐ : ∀ w o, (o,w) ⊨ p → (o,w) ⊨ Jₐ
-parameter evt_Jₐ  : ∀ w o w' o' e,
-                          (o,w) ⊨ Jₐ →
-                          (o,w) ⊨ cs₀ e →
-                          (o,w) ⊨ fs₀ e →
-                          A e (o,w) (o',w') →
-                          (o',w') ⊨ Jₐ
+-- parameter init_Jₐ : ∀ w o, (o,w) ⊨ p → (o,w) ⊨ Jₐ
+-- parameter evt_Jₐ  : ∀ w o w' o' e,
+--                           (o,w) ⊨ Jₐ →
+--                           (o,w) ⊨ cs₀ e →
+--                           (o,w) ⊨ fs₀ e →
+--                           A e (o,w) (o',w') →
+--                           (o',w') ⊨ Jₐ
 
-parameter SIM₀ : ∀ v o, (o,v) ⊨ q → ∃ w, (o,w) ⊨ p ∧ (o,w,v) ⊨ J
-parameter SIM
-: ∀ w v o v' o' ce,
-  (o,w,v) ⊨ J →
-  (o,w) ⊨ Jₐ →
-  (o,v) ⊨ cs₁ ce →
-  (o,v) ⊨ fs₁ ce →
-  C ce (o,v) (o',v') →
-  ∃ ae w', (o',w',v') ⊨ J ∧
-           ref ae ce ∧
-           (o,w) ⊨ cs₀ ae ∧
-           (o,w) ⊨ fs₀ ae ∧
-           A ae (o,w) (o',w')
+structure refinement :=
+  (SIM₀ : ∀ v o, (o,v) ⊨ q → ∃ w, (o,w) ⊨ p ∧ (o,w,v) ⊨ J)
+  (SIM : ∀ cev w v o v' o',
+    (o,w,v) ⊨ J →
+    m₁.effect cev (o,v) (o',v') →
+    ∃ aev w', ref aev cev ∧
+             m₀.effect aev (o,w) (o',w') ∧
+             (o',w',v') ⊨ J )
+  (ANIM : ∀ (e : aevt) (sch : tvar (option aevt)) (o v w),
+    many_to_many_po'
+      (subtype _)
+      (SPEC₁ v o ⋀ SPEC₀.saf' w o sch ⋀ ◻(J ! ⦃o,w,v⦄))
+      (wit e)
+      (λ e', ce e') (ae e)
+      ⦃o,v⦄ ⦃o,w⦄)
 
 section obligations
 
 parameters (v : tvar β) (o : tvar γ)
 parameters (Γ : cpred)
 
+parameter Href : refinement
+
 parameters β γ
-variable Hpo : ∀ (e : aevt) (w : tvar α) (sch : tvar aevt),
-  many_to_many_po'
-    (subtype (ref e))
-    (SPEC₁ v o ⋀ SPEC₀.saf' w o sch ⋀ ◻(J ! ⦃o,w,v⦄))
-    (wit e)
-    (λ e', ce e') (ae e)
-    ⦃o,v⦄ ⦃o,w⦄
 parameters {β γ}
 
 section conc_sch
 
-parameters (sch_c : tvar cevt)
+parameters (sch_c : tvar (option cevt))
 
-variable (sch_a : tvar aevt)
+variable (sch_a : tvar (option aevt))
 
 section SPEC₂
 variable H : Γ ⊢ SPEC₂ v o sch_c
 
 open prod temporal.prod
 
-def Next_a : act $ γ × aevt × α :=
-λ σ σ',
-∃ e, σ.2.1 = e ∧
-      map_right snd σ ⊨ cs₀ e ∧
-      map_right snd σ ⊨ fs₀ e ∧
-      (A e on map_right snd) σ σ'
+-- def Next_a : act $ γ × aevt × α :=
+-- λ σ σ',
+-- ∃ e, σ.2.1 = e ∧
+--       map_right snd σ ⊨ cs₀ e ∧
+--       map_right snd σ ⊨ fs₀ e ∧
+--       (A e on map_right snd) σ σ'
 
-def Next_c : act $ γ × cevt × β :=
-λ σ σ',
-∃ e, σ.2.1 = e ∧
-      map_right snd σ ⊨ cs₁ e ∧
-      map_right snd σ ⊨ fs₁ e ∧
-      (C e on map_right snd) σ σ'
+-- def Next_c : act $ γ × cevt × β :=
+-- λ σ σ',
+-- ∃ e, σ.2.1 = e ∧
+--       map_right snd σ ⊨ cs₁ e ∧
+--       map_right snd σ ⊨ fs₁ e ∧
+--       (C e on map_right snd) σ σ'
 
 section J
 def J' : pred' (γ × (aevt × α) × (cevt × β)) :=
 J ! ⟨ prod.map_right $ prod.map prod.snd prod.snd ⟩ ⋀
 ⟨ λ ⟨_, a, c⟩, ref a.1 c.1 ⟩
 
-def JJₐ : pred' (γ × aevt × α) :=
-Jₐ ! ⟨ prod.map_right snd ⟩
+-- def JJₐ : pred' (γ × aevt × α) :=
+-- Jₐ ! ⟨ prod.map_right snd ⟩
 
 def p' : pred' (γ × aevt × α) :=
 p ! ⟨prod.map_right prod.snd⟩
@@ -145,70 +152,74 @@ q ! ⟨prod.map_right prod.snd⟩
 end J
 variable w : tvar α
 open function
-include inh_aevt inh_α
-noncomputable def Wx₀_f : tvar (β → γ → aevt × α) :=
-λ v o, ε w : aevt × _, (o,w.2) ⊨ p ∧ (o,w.2,v) ⊨ J
+include inh_aevt
+-- def Wx₀_f : tvar (β → γ → aevt × α → Prop) :=
+-- λ v o (w : aevt × _), (o,w.2) ⊨ p ∧ (o,w.2,v) ⊨ J
 
-noncomputable def Wx₀ : tvar (aevt × α) :=
-Wx₀_f v o
+-- @[simp]
+-- def Wx₀ : tvar (option aevt × α → Prop) :=
+-- [| v o , λ (w : option aevt × _), (o,w.2) ⊨ p |]
 
-noncomputable def Wf_f : tvar (cevt → β → γ → γ → aevt × α → aevt × α) :=
-⟪ℕ, λ ce v' o o' (w : _ × _),
-      ε w' : aevt × α,
-             (o',w'.2,v') ⊨ J ∧
-             ref w'.1 ce ∧
-             (o,w.2) ⊨ cs₀ w'.1 ∧
-             (o,w.2) ⊨ fs₀ w'.1 ∧
-             A w'.1 (o,w.2) (o',w'.2) ⟫
+-- def Wf_f : tvar (option cevt → β → γ → γ → option aevt × α → option aevt × α → Prop) :=
+-- ⟪ℕ, λ ce v' o o' (w : _ × _) (w' : option aevt × α),
+--              (o',w'.2,v') ⊨ J ∧
+--              ref w'.1 ce ∧
+--              -- (o,w.2) ⊨ cs₀ w'.1 ∧
+--              -- (o,w.2) ⊨ fs₀ w'.1 ∧
+--              m₀.effect w'.1 (o,w.2) (o',w'.2) ⟫
+--              -- A w'.1 (o,w.2) (o',w'.2) ⟫
 
-noncomputable def Wf : tvar (aevt × α → aevt × α) :=
-Wf_f sch_c (⊙v) o (⊙o)
+-- @[simp]
+-- def Wf : tvar (option aevt × α → option aevt × α → Prop) :=
+-- ⟪ℕ, λ (cev : option cevt) o o' (w w' : option aevt × α),
+--              ref w'.1 cev ∧
+--              -- (o,w.2) ⊨ cs₀ w'.1 ∧
+--              -- (o,w.2) ⊨ fs₀ w'.1 ∧
+--              m₀.effect w'.1 (o,w.2) (o',w'.2) ⟫
+--  sch_c o (⊙o)
 
-noncomputable def Wtn (w : tvar (aevt × α)) :=
-w ≃ Wx₀ ⋀ ◻(⊙w ≃ Wf w)
+-- lemma Wx₀_def' (σ : ℕ)
+-- : σ ⊨ Wx₀ =
+--   ε w : _ × α, (σ ⊨ o,w.2) ⊨ p ∧ (σ ⊨ o,w.2,σ ⊨ v) ⊨ J :=
+-- by repeat { unfold_coes <|> simp [Wx₀,Wx₀_f] }
 
-lemma Wx₀_def' (σ : ℕ)
-: σ ⊨ Wx₀ =
-  ε w : _ × α, (σ ⊨ o,w.2) ⊨ p ∧ (σ ⊨ o,w.2,σ ⊨ v) ⊨ J :=
-by repeat { unfold_coes <|> simp [Wx₀,Wx₀_f] }
+-- @[simp,predicate]
+-- lemma Wx₀_def (σ : ℕ) (a b)
+-- : (a,b) = σ ⊨ Wx₀ ↔
+--   a = (ε w : _ × α,    (σ ⊨ o,w.2) ⊨ p ∧ (σ ⊨ o,w.2,σ ⊨ v) ⊨ J).fst ∧
+--   b = (ε w : aevt × α, (σ ⊨ o,w.2) ⊨ p ∧ (σ ⊨ o,w.2,σ ⊨ v) ⊨ J).snd :=
+-- by repeat { unfold_coes <|> simp [Wx₀,Wx₀_f,ext] }
 
-@[simp,predicate]
-lemma Wx₀_def (σ : ℕ) (a b)
-: (a,b) = σ ⊨ Wx₀ ↔
-  a = (ε w : _ × α,    (σ ⊨ o,w.2) ⊨ p ∧ (σ ⊨ o,w.2,σ ⊨ v) ⊨ J).fst ∧
-  b = (ε w : aevt × α, (σ ⊨ o,w.2) ⊨ p ∧ (σ ⊨ o,w.2,σ ⊨ v) ⊨ J).snd :=
-by repeat { unfold_coes <|> simp [Wx₀,Wx₀_f,ext] }
-
-lemma Wf_def' (σ : ℕ) (w)
-: σ ⊨ Wf ⦃sch_a,w⦄ =
-  ε w' : _ × α,
-         (succ σ ⊨ o,w'.2,succ σ ⊨ v) ⊨ J ∧
-               ref w'.1 (σ ⊨ sch_c) ∧
-               (σ ⊨ o,σ ⊨ w) ⊨ cs₀ w'.1 ∧
-               (σ ⊨ o,σ ⊨ w) ⊨ fs₀ w'.1 ∧
-               A w'.1 (σ ⊨ o,σ ⊨ w) (succ σ ⊨ o,w'.2) :=
-by repeat { unfold_coes <|> simp [Wf,Wf_f] }
+-- lemma Wf_def' (σ : ℕ) (w)
+-- : σ ⊨ Wf ⦃sch_a,w⦄ =
+--   ε w' : _ × α,
+--          (succ σ ⊨ o,w'.2,succ σ ⊨ v) ⊨ J ∧
+--                ref w'.1 (σ ⊨ sch_c) ∧
+--                (σ ⊨ o,σ ⊨ w) ⊨ cs₀ w'.1 ∧
+--                (σ ⊨ o,σ ⊨ w) ⊨ fs₀ w'.1 ∧
+--                A w'.1 (σ ⊨ o,σ ⊨ w) (succ σ ⊨ o,w'.2) :=
+-- by repeat { unfold_coes <|> simp [Wf,Wf_f] }
 
 
-@[simp,predicate]
-lemma Wf_def (σ : ℕ) (sch_a w) (a b)
-: (a,b) = (σ ⊨ Wf) (sch_a,w) ↔
-  a = (ε w' : _ × α,
-         (succ σ ⊨ o,w'.2,succ σ ⊨ v) ⊨ J ∧
-               ref w'.1 (σ ⊨ sch_c) ∧
-               (σ ⊨ o,w) ⊨ cs₀ w'.1 ∧
-               (σ ⊨ o,w) ⊨ fs₀ w'.1 ∧
-               A w'.1 (σ ⊨ o,w) (succ σ ⊨ o,w'.2)).1 ∧
-  b = (ε w' : aevt × α,
-         (succ σ ⊨ o,w'.2,succ σ ⊨ v) ⊨ J ∧
-               ref w'.1 (σ ⊨ sch_c) ∧
-               (σ ⊨ o,w) ⊨ cs₀ w'.1 ∧
-               (σ ⊨ o,w) ⊨ fs₀ w'.1 ∧
-               A w'.1 (σ ⊨ o,w) (succ σ ⊨ o,w'.2)).2 :=
-by repeat { unfold_coes <|> simp [Wf,Wf_f,ext] }
+-- @[simp,predicate]
+-- lemma Wf_def (σ : ℕ) (sch_a w) (a b)
+-- : (a,b) = (σ ⊨ Wf) (sch_a,w) ↔
+--   a = (ε w' : _ × α,
+--          (succ σ ⊨ o,w'.2,succ σ ⊨ v) ⊨ J ∧
+--                ref w'.1 (σ ⊨ sch_c) ∧
+--                (σ ⊨ o,w) ⊨ cs₀ w'.1 ∧
+--                (σ ⊨ o,w) ⊨ fs₀ w'.1 ∧
+--                A w'.1 (σ ⊨ o,w) (succ σ ⊨ o,w'.2)).1 ∧
+--   b = (ε w' : aevt × α,
+--          (succ σ ⊨ o,w'.2,succ σ ⊨ v) ⊨ J ∧
+--                ref w'.1 (σ ⊨ sch_c) ∧
+--                (σ ⊨ o,w) ⊨ cs₀ w'.1 ∧
+--                (σ ⊨ o,w) ⊨ fs₀ w'.1 ∧
+--                A w'.1 (σ ⊨ o,w) (succ σ ⊨ o,w'.2)).2 :=
+-- by repeat { unfold_coes <|> simp [Wf,Wf_f,ext] }
 
-variable valid_witness
-: Γ ⊢ Wtn ⦃sch_a,w⦄
+-- variable valid_witness
+-- : Γ ⊢ Wtn ⦃sch_a,w⦄
 
 -- lemma abstract_sch (e : aevt)
 -- : Γ ⊢ sch_a ≃ e ⋀ cs₀ e ! ⦃o,w⦄ ⋀ fs₀ e ! ⦃o,w⦄ ⋀ ⟦ o,w | A e ⟧ ≡
@@ -271,88 +282,99 @@ section Simulation_POs
 -- end
 
 -- omit H
-abbreviation ref' : tvar (aevt → cevt → Prop) :=
+abbreviation ref' : tvar (option aevt → option cevt → Prop) :=
 ref
 
-include valid_witness init_Jₐ evt_Jₐ
-include SIM₀ SIM H
+@[simp]
+def Next₀ : act (γ × α × option aevt) :=
+λ ⟨o,w,sch_a⟩ ⟨o',w',_⟩, ∃ e, sch_a = e ∧ m₀.effect e (o,w) (o',w')
+
+-- include valid_witness -- init_Jₐ evt_Jₐ
+include H Href
+-- set_option pp.implicit true
 
 lemma J_inv_in_w'
-: Γ ⊢ ◻(J ! ⦃o,w,v⦄ ⋀ Jₐ ! ⦃o,w⦄) :=
+: Γ ⊢ ∃∃ w, ◻(J ! ⦃o,w,v⦄) ⋀ SPEC₀.saf' w o sch_a :=
 begin [temporal]
-  simp [Wtn,SPEC₂] at valid_witness H,
-  cases valid_witness with h₀ h₀,
-  casesm* _ ⋀ _,
-  apply induct _ _ _ _,
-  { select H₀ : ◻p_exists _,
-    henceforth! at h₀_1 H₀ ⊢,
-    explicit'
-      with H₀ h₀_1 SIM evt_Jₐ
-    { intros h hJₐ,
-      casesm* [_ ∧ _,Exists _],
-      have : (o', w', v') ⊨ J ∧
-             (o,w) ⊨ cs₀ sch_a' ∧ (o,w) ⊨ fs₀ sch_a' ∧
-             A sch_a' (o, w) (o', w'),
-      { subst H₀_w, subst w', subst sch_a',
-        apply_epsilon_spec,
-        simp,
-        apply SIM ; solve_by_elim },
-      split, tauto,
-      casesm* _ ∧ _,
-      apply evt_Jₐ ; apply hJₐ <|> solve_by_elim } },
-  { select Hw : _ ≃ temporal.many_to_many.Wx₀,
-    select Hq : q ! _,
-    clear_except Hw SIM₀ Hq init_Jₐ,
-    explicit' with Hw SIM₀ Hq init_Jₐ
-    { cases Hw, subst w, apply_epsilon_spec,
-      simp, tauto, } },
+  -- select_witness w : temporal.many_to_many.Wtn w
+  --   with Hw using J ! ⦃o,w.snd,v⦄,
+  unfold SPEC₂ mch.spec_sch at H, casesm* _ ⋀ _,
+
+  select_witness w : m₀.init ! ⦃o,w⦄ ⋀ ◻ ⟦ o,w,sch_a | temporal.many_to_many.Next₀ ⟧
+    -- with h₀ h₁
+    using (J ! ⦃o,w,v⦄)
+  { ext, admit, -- simp_coe [to_fun_var'],
+    -- simp only with lifted_fn,
+    -- congr, funext, transitivity, apply to_fun_var'_lift₂,
+    -- -- congr,
+    -- simp [to_fun_var'_coe] with lifted_fn,
+    -- congr, rw to_fun_var'_id,
+    -- refl,
+    },
+  explicit' with a
+  { apply Href.SIM₀, assumption },
+  -- simp [SPEC₂] at H,
+  -- rw henceforth_next_intro,
+  -- dsimp [SPEC₀.saf'],
+  -- -- cases valid_witness with h₀ h₀,
+  -- casesm* _ ⋀ _,
+  -- intros,
+  -- t_induction,
+  -- { -- select Hw : _ ≃ temporal.many_to_many.Wx₀,
+  --   select Hq : q ! _,
+  --   have SIM₀ := Href.SIM₀,
+  --   explicit' with SIM₀ Hq
+  --   { {  },
+  --     simp, tauto, } },
+  { select H₀ : p_exists _,
+    -- henceforth! at h₀_1 H₀ ⊢,
+    explicit' [Next₀] with H₀
+    { intros h hJ,
+      -- casesm* [_ ∧ _,Exists _],
+      -- type_check cs₀,
+      -- have : (o', h', v') ⊨ J ∧
+      --        (o,w) ⊨ cs₀ sch_a' ∧ (o,w) ⊨ fs₀ sch_a' ∧
+      --        A sch_a' (o, w) (o', w'),
+      -- { subst H₀_w, subst w', subst sch_a',
+      --   apply_epsilon_spec,
+      --   simp,
+      --   apply SIM ; solve_by_elim },
+      -- split, tauto,
+      -- casesm* _ ∧ _,
+      -- apply evt_Jₐ ; apply hJₐ <|> solve_by_elim
+      } },
 end
 
-lemma J_inv_in_w
-: Γ ⊢ ◻(J ! ⦃o,w,v⦄) :=
-begin [temporal]
-  cases temporal.many_to_many.J_inv_in_w' _ H _ valid_witness,
-  assumption
-end
+-- lemma J_inv_in_w
+-- : Γ ⊢ ◻(J ! ⦃o,w,v⦄) :=
+-- begin [temporal]
+--   cases temporal.many_to_many.J_inv_in_w' _ H _ valid_witness,
+--   assumption
+-- end
 
-lemma abs_J_inv_in_w
-: Γ ⊢ ◻(Jₐ ! ⦃o,w⦄) :=
-begin [temporal]
-  cases temporal.many_to_many.J_inv_in_w' _ H _ valid_witness,
-  assumption
-end
+-- lemma abs_J_inv_in_w
+-- : Γ ⊢ ◻(Jₐ ! ⦃o,w⦄) :=
+-- begin [temporal]
+--   cases temporal.many_to_many.J_inv_in_w' _ H _ valid_witness,
+--   assumption
+-- end
 
 lemma witness_imp_SPEC₀_saf
 : Γ ⊢ SPEC₀.saf' w o sch_a :=
 begin [temporal]
-  have hJ  := temporal.many_to_many.J_inv_in_w sch_a H w valid_witness ,
-  have hJₐ := temporal.many_to_many.abs_J_inv_in_w sch_a H w valid_witness,
-  simp [SPEC₀.saf',SPEC₂,Wtn] at valid_witness ⊢ H,
-  casesm* _ ⋀ _,
+  simp [SPEC₀.saf',Wtn] at ⊢ valid_witness,
+  cases valid_witness with H₀ H₁,
   split,
-  { clear SIM,
-    henceforth at hJ,
-    select Hw : _ ≃ temporal.many_to_many.Wx₀,
-    select h' : q ! _,
-    explicit' with Hw h'
-    { cases Hw, subst w,
-      apply_epsilon_spec,
-      simp, solve_by_elim, } },
-  { clear SIM₀,
-    select h : ◻(_ ≃ _),
-    select h' : ◻(p_exists _),
-    henceforth! at h h' ⊢ hJ hJₐ,
-    explicit' with h h' hJ hJₐ
-    { cases h, subst w', subst sch_a',
-      casesm* [_ ∧ _,Exists _],
-      subst h'_w,
-      apply_epsilon_spec, simp,
-      apply SIM ; solve_by_elim, } },
+  explicit' with H₀
+  { tauto, },
+  henceforth!,
+  explicit' with H₁
+  { tauto, },
 end
 
 omit H
-parameters p q cs₁ fs₁
-include Hpo p
+parameters m₀ m₁
+include Href
 omit valid_witness
 
 lemma SPEC₂_imp_SPEC₁
@@ -368,36 +390,37 @@ begin [temporal]
 end
 
 section
-omit Hpo
-include valid_witness fs₁ cs₁ Γ H
+omit Href
+include valid_witness Γ H
 -- #check w
 -- noncomputable def sch_w : tvar aevt :=
 -- ⟪ ℕ, λ (w w' : α), ε ae, A ae w w' ⟫ w (⊙w)
 
-lemma sch_w_spec
-: Γ ⊢ ◻(ref' (⊙sch_a) sch_c) :=
-begin [temporal]
-  have hJ  := temporal.many_to_many.J_inv_in_w _ H _ valid_witness,
-  have hJₐ := temporal.many_to_many.abs_J_inv_in_w _ H _ valid_witness,
-  simp [Wtn,SPEC₂] at valid_witness H,
-  cases valid_witness with Hw' Hw,
-  cases H with H H₀,
-  cases H with H₁ H₂,
-  henceforth! at Hw ⊢ hJ hJₐ H₂,
-  explicit' with Hw hJ hJₐ H₂
-  { cases Hw, subst sch_a', casesm* [_∧_,Exists _],
-    subst sch_c, apply_epsilon_spec,
-    simp, solve_by_elim, },
-end
+-- lemma sch_w_spec
+-- : Γ ⊢ ◻(ref' (⊙sch_a) sch_c) :=
+-- begin [temporal]
+--   have hJ  := temporal.many_to_many.J_inv_in_w _ H _ valid_witness,
+--   have hJₐ := temporal.many_to_many.abs_J_inv_in_w _ H _ valid_witness,
+--   simp [Wtn,SPEC₂] at valid_witness H,
+--   cases valid_witness with Hw' Hw,
+--   cases H with H H₀,
+--   cases H with H₁ H₂,
+--   henceforth! at Hw ⊢ hJ hJₐ H₂,
+--   explicit' with Hw hJ hJₐ H₂
+--   { cases Hw, subst sch_a', casesm* [_∧_,Exists _],
+--     subst sch_c, apply_epsilon_spec,
+--     simp, solve_by_elim, },
+-- end
 
 end
 
 include H valid_witness
-lemma H_C_imp_A (e : cevt) (e' : aevt)
-  -- (Hsim : ref e' e)
+
+lemma H_C_imp_A (e : option cevt) (e' : option aevt)
+  (Hsim : ref e' e)
 : Γ ⊢ ◻(sch_c ≃ ↑e ⟶ ⊙sch_a ≃ ↑e' ⟶
-        cs₁ e ! ⦃o,v⦄ ⋀ fs₁ e ! ⦃o,v⦄ ⋀ ⟦ o,v | C e ⟧ ⟶
-        cs₀ e' ! ⦃o,w⦄ ⋀ fs₀ e' ! ⦃o,w⦄ ⋀ ⟦ o,w | A e' ⟧) :=
+        ⟦ o,v | Next₁ e ⟧ ⟶
+        ⟦ o,w | Next₀ e' ⟧) :=
 begin [temporal]
   have hJ := temporal.many_to_many.J_inv_in_w sch_a H w valid_witness,
   have hJₐ := temporal.many_to_many.abs_J_inv_in_w sch_a H w valid_witness,
@@ -414,16 +437,15 @@ begin [temporal]
     apply_epsilon_spec,
     simp, apply SIM ; solve_by_elim, },
 end
+
 omit valid_witness H
-/- latest idea: sch_a should be part of concrete state?
--/
 
 lemma Hpo' (e : aevt)
 : many_to_many_po'
-     (subtype (ref e)) (SPEC₂ v o sch_c ⋀ Wtn ⦃sch_a,w⦄ ⋀ ◻(J ! ⦃o,w,v⦄))
+     _ (SPEC₂ v o sch_c ⋀ Wtn ⦃sch_a,w⦄ ⋀ ◻(J ! ⦃o,w,v⦄))
      (wit e)
      (λ i, ce' i e) (ae e)
-     ⦃o,v,sch_c,sch_a⦄ ⦃o,w⦄
+     ⦃⦃o,v⦄,sch_c,sch_a⦄ ⦃o,w⦄
 :=
 begin
   have
@@ -433,14 +455,14 @@ begin
       ◻(J ! ⦃o,w,v⦄),
   begin [temporal]
     simp, intros h₀ h₁ h₂, split*,
-    { apply temporal.many_to_many.SPEC₂_imp_SPEC₁ Hpo _ ; try { solve_by_elim }, },
+    { apply temporal.many_to_many.SPEC₂_imp_SPEC₁ _ _ ; try { solve_by_elim }, },
     { apply temporal.many_to_many.witness_imp_SPEC₀_saf _ h₀ _ h₁, },
     { solve_by_elim }
   end,
   constructor,
   iterate 3
-  { cases (Hpo e w sch_a),
-    simp at *,
+  { cases (Href.ANIM e sch_a o v w),
+    simp! [ce',mch.event'] at *,
     transitivity,
     { apply this },
     { assumption } },
@@ -451,41 +473,43 @@ begin
     select Hw : temporal.many_to_many.Wtn _,
     select hJ : ◻(J ! _),
     select H  : temporal.many_to_many.SPEC₂ _ _ _,
-    have := temporal.many_to_many.H_C_imp_A _ _ _ _ Hw x e
-    ; try { solve_by_elim <|> apply temporal.many_to_many.sch_w_spec },
+    have := temporal.many_to_many.H_C_imp_A _ H w Hw _ e x.2,
     cases H with H H₀,
     cases H with H₁ H₂,
-    clear_except this SIM₀ SIM Hw hJ H₂,
+    clear_except this Href SIM₀ SIM Hw hJ H₂,
     simp [Wtn] at Hw, cases Hw with Hw' Hw,
-    henceforth! at ⊢ this Hw hJ H₂,
-    explicit' with this Hw hJ H₂
-    { intros, cases Hw, simp only [ce'._match_2,ce'._match_1] at *,
-      casesm* [_ ∧ _, Exists _],
-      apply this _ _ ; tauto <|> cc, },
+    henceforth! at ⊢ Hw hJ H₂ this,
+    explicit' [mch.event'] with this Hw hJ H₂
+    { dsimp [ce',mch.event'], cases Hw,
+      intros,
+      casesm* [_ ∧ _, Exists _, sch_c = _],
+      specialize this _ _ _ ; try { assumption },
+      simp [and_assoc,*], exact this, },
   end
 end
 
 end Simulation_POs
 
-include H SIM₀ SIM Hpo init_Jₐ evt_Jₐ
+include H Href
 
 lemma sched_ref (i : aevt) -- (w : tvar (aevt × α))
+ (hJ : Γ ⊢ ◻(J ! ⦃o,w,v⦄))
  (Hw : Γ ⊢ Wtn ⦃sch_a,w⦄)
- (h : Γ ⊢ ∀∀ j, ref i j ⟶ sched (cs₁ j ! ⦃o,v⦄) (fs₁ j ! ⦃o,v⦄) (sch_c ≃ ↑j ⋀ ⟦ o,v | C j ⟧))
+ (h : Γ ⊢ ∀∀ j : cevt, ref ↑i ↑j ⟶ sched (cs₁ j ! ⦃o,v⦄) (fs₁ j ! ⦃o,v⦄) (sch_c ≃ some j ⋀ ⟦ o,v | C j ⟧))
 : Γ ⊢ sched (cs₀ i ! ⦃o,w⦄) (fs₀ i ! ⦃o,w⦄) ⟦ o,w | A i ⟧ :=
 begin [temporal]
-  have hJ : ◻(J ! ⦃o,w,v⦄),
-  { apply temporal.many_to_many.J_inv_in_w ; solve_by_elim },
-  apply splitting (Hpo i w sch_a) _ _,
-  { split, split,
-    apply temporal.many_to_many.SPEC₂_imp_SPEC₁ Hpo ; solve_by_elim,
-    apply temporal.many_to_many.witness_imp_SPEC₀_saf ; solve_by_elim,
-    solve_by_elim },
-  intro ce, cases ce with ce Hce,
+  -- have hJ : ◻(J ! ⦃o,w,v⦄),
+  -- { apply temporal.many_to_many.J_inv_in_w ; solve_by_elim },
+  apply splitting (Href.ANIM i sch_a o v w) _ _,
+  { split*,
+    apply temporal.many_to_many.SPEC₂_imp_SPEC₁ _ ; assumption,
+    apply temporal.many_to_many.witness_imp_SPEC₀_saf ; assumption,
+    assumption },
+  intro cev, cases cev with cev Hce,
   simp only, intros H₀ H₁,
-  replace h := h ce Hce H₀ H₁,
+  replace h := h cev Hce H₀ H₁,
   revert h,
-  monotonicity!, clear Hpo,
+  monotonicity!,
   explicit'
   { intros, tauto },
 end
@@ -499,49 +523,31 @@ end
 lemma many_to_many
 : Γ ⊢ ∃∃ w, SPEC₀ w o :=
 begin [temporal]
-  apply p_exists_partial_intro _ (proj $ @pair.snd aevt α) _ _,
-  select_witness w : temporal.many_to_many.Wtn w with Hw,
-  cases w with sch_a w,
-  have this := H, revert this,
-  dsimp [SPEC₀,SPEC₁],
-  -- have H' := temporal.many_to_many.H' , -- o sch,
-  apply ctx_p_and_p_imp_p_and' _ _,
-  apply ctx_p_and_p_imp_p_and' _ _,
-  { clear_except SIM₀ Hw,
-    simp [Wtn,SPEC₂] at Hw,
-    casesm _ ⋀ _,
-    select Hw : (_ ≃ temporal.many_to_many.Wx₀),
-    explicit'  with Hw
-    { intro, cases Hw,
-      subst w, apply_epsilon_spec,
-      simp, solve_by_elim, }, },
-  { clear_except SIM SIM₀ Hw H init_Jₐ evt_Jₐ,
-    have hJ := temporal.many_to_many.J_inv_in_w _ H _ Hw,
-    have hJₐ := temporal.many_to_many.abs_J_inv_in_w _ H _ Hw,
-    clear H,
-    simp [Wtn,SPEC₂] at Hw,
-    casesm _ ⋀ _,
-    monotonicity!,
-    simp, intros ce h₀ h₁ h₂ h₃,
-    select Hw : ◻(_ ≃ _),
-    henceforth at Hw hJ hJₐ,
-    explicit' with h₀ h₁ h₂ h₃ hJ hJₐ Hw
-    { cases Hw, subst w', subst ce,
-      apply_epsilon_spec,
-      simp, apply SIM ; clear SIM,
-      repeat { solve_by_elim }, }, },
-  { intros h i,
-    have REF := temporal.many_to_many.sched_ref Hpo sch_a H w i Hw,
-    clear_except REF h,
-    apply REF, intros,
-    apply h ; assumption, },
+  apply p_exists_partial_intro _ (proj $ @pair.snd (option aevt) α) _ _,
+  -- replace H := H.left,
+  cases H.left with H₀ H₁,
+  select_witness w : temporal.many_to_many.Wtn w
+    with Hw using J ! ⦃o,w.snd,v⦄,
+  explicit' [Wx₀] with H₀
+  { apply Href.SIM₀ _ _ H₀, },
+  explicit' [Wf] with H₁
+  { simp_intros b hJ [and_assoc],
+    have := Href.SIM _ _ _ _ _ _ hJ H₁,
+    tauto, }, -- a ∧ a ↔ a
+  existsi w,
+  { apply m₀.spec_of_spec_saf_sch _ (⊙w.fst),
+    apply temporal.many_to_many.witness_imp_SPEC₀_saf _ H,
+    revert Hw, simp,
+    intro, apply temporal.many_to_many.sched_ref w.fst H w.snd x,
+    assumption, simp *, introv H',
+    apply H.right, },
 end
 end SPEC₂
 end conc_sch
 
 section refinement_SPEC₂
-include SIM₀ SIM wit Hpo inh_aevt inh_α init_Jₐ evt_Jₐ
-parameters cs₁ fs₁ cs₀ fs₀
+include Href wit inh_aevt
+parameters m₀ m₁
 
 lemma refinement_SPEC₂
 : Γ ⊢ (∃∃ sch_c, SPEC₂ v o sch_c) ⟶ (∃∃ a, SPEC₀ a o) :=
@@ -553,32 +559,29 @@ end
 
 end refinement_SPEC₂
 
-open nat function set
+open nat function set scheduling
 include inh_cevt
 
-variables [schedulable cevt]
+variables [encodable cevt]
 
 lemma refinement_SPEC₁
 : SPEC₁ v o ⟹ (∃∃ sch, SPEC₂ v o sch) :=
 assume Γ,
-sch_intro _ _ _ _ _ _
+sch_intro _ _ _
 
 end obligations
 open function
-include SIM₀ SIM inh_cevt inh_aevt inh_α init_Jₐ evt_Jₐ
-lemma refinement {o : tvar γ} [schedulable cevt]
-  (h :   ∀ (v : tvar β) (e : aevt) (w : tvar α) (sch_a : tvar aevt),
-    many_to_many_po' (subtype (ref e)) (SPEC₁ v o ⋀ SPEC₀.saf' w o sch_a ⋀ ◻(J ! ⦃o,w,v⦄)) (wit e)
-      (λ (e' : subtype (ref e)), ce ↑e') (ae e)
-      ⦃o,v⦄ ⦃o,w⦄)
+include J wit inh_cevt inh_aevt
+
+lemma refinement' {o : tvar γ} [encodable cevt]
+  (h : refinement)
 : (∃∃ c, SPEC₁ c o) ⟹ (∃∃ a, SPEC₀ a o) :=
 begin [temporal]
-  transitivity (∃∃ c sch, SPEC₂ q C cs₁ fs₁ c o sch),
+  transitivity (∃∃ c (sch : tvar (option cevt)), SPEC₂ c o sch),
   { apply p_exists_p_imp_p_exists ,
     intro v,
     apply temporal.many_to_many.refinement_SPEC₁, },
   { simp, intros c sch Hspec,
-    specialize h c,
     apply temporal.many_to_many.refinement_SPEC₂ c o Γ h,
     existsi sch, exact Hspec, },
 end
